Resyncinc traces with Paco

Trace.v
@@ -226,22 +226,23 @@ Lemma TraceAppNone :
   forall {A} (T : TraceOf A),
     TraceEq T (T^None).
 Proof.
-  cofix COFIX. intros. rewrite idTrace_eq. destruct T.
+  intro A. pcofix COFIX. intros; pfold. rewrite idTrace_eq. destruct T.
   - simpl. constructor.
-  - simpl. constructor. apply COFIX. 
+  - simpl. constructor. right. apply COFIX.
 Qed.
 
 Lemma TraceAppAssoc :
   forall A (T1 T2 : TraceOf A) TO,
     T1 ^ Some (T2 ^ TO) ~= (T1 ^ Some T2) ^ TO.
 Proof.
-  cofix COFIX.
-  intros.
+  intro A. pcofix COFIX.
+  intros; pfold.
   destruct T1.
-  - rewrite idTrace_eq.  rewrite idTrace_eq at 1. simpl.  reflexivity.
-  - rewrite idTrace_eq.  rewrite (idTrace_eq (notfinished a T1 ^ Some (T2 ^ TO))). simpl. 
-    constructor. 
-    apply COFIX. 
+  - rewrite idTrace_eq.  rewrite idTrace_eq at 1. simpl.
+    constructor. left. apply paco2_mon_bot with TraceEq_gen; [| auto]. apply TraceEqRefl.
+  - rewrite idTrace_eq.  rewrite (idTrace_eq (notfinished a T1 ^ Some (T2 ^ TO))). simpl.
+    constructor.
+    right. apply COFIX.
 Qed.
 
 (* TracePrefix T1 T2 says T2 is a prefix of T1. *)
@@ -304,11 +305,18 @@ Add Parametric Morphism A: (@TracePrefix A)
 Proof.
   exact (@TracePrefixEq A).                                                                                     Qed.                            
                              
+Inductive ForallTrace_gen {A : Type} (P : A -> Prop) R : TraceOf A -> Prop :=
+| Forall_finished : forall a,
+    P a -> ForallTrace_gen P R (finished a)
+| Forall_notfinished : forall a T',
+    P a -> R T' -> ForallTrace_gen P R (notfinished a T').
+Hint Constructors ForallTrace_gen : core.
 
-CoInductive ForallTrace {A:Type} (P:A -> Prop) : TraceOf A -> Prop :=
-| Forall_finished : forall a, P a -> ForallTrace P (finished a)
-| Forall_notfinished : forall a T', P a -> ForallTrace P T' -> ForallTrace P (notfinished a T')
-.
+Definition ForallTrace {A} (P : A -> Prop) (T : TraceOf A) :=
+  paco1 (ForallTrace_gen P) bot1 T.
+Hint Unfold ForallTrace : core.
+Lemma ForallTrace_mon A P : monotone1 (@ForallTrace_gen A P). Proof. pmonauto. Qed.
+Hint Resolve ForallTrace_mon : paco.
 
 Lemma ForallInTrace :
   forall {A} (f:A->Prop) T t,
@@ -316,14 +324,14 @@ Lemma ForallInTrace :
     ForallTrace f T ->
     f t.
 Proof.
-  intros. induction H; inversion H0; auto.
+  intros. induction H; pinversion H0; auto.
 Qed.
 
 Lemma ForallTraceTautology :
   forall {A} (P:A->Prop) (T:TraceOf A),
     (forall a, P a) -> ForallTrace P T.
 Proof.
-  cofix COFIX. intros. destruct T;constructor;auto.
+  intros A P. pcofix COFIX. intros; pfold. destruct T;constructor;auto.
 Qed.
 
 Lemma ForallTraceEq:
@@ -332,11 +340,11 @@ Lemma ForallTraceEq:
     ForallTrace f T1 ->
     ForallTrace f T2. 
 Proof.
-  cofix COFIX.  intros. 
-  destruct H. 
-  inv H0. 
+  intros A f. pcofix COFIX. intros T1 T2 H H0; pfold.
+  pdestruct H.
+  inv H0.
   - constructor. auto.
-  - inv H0. constructor.  auto. eapply COFIX; eauto. 
+  - inv H0. constructor. auto. right. eapply COFIX; eauto.
 Qed.
 
 Add Parametric Morphism A (f:A->Prop) : (@ForallTrace A f)
